Azurite/AzNat/Conversion.lean
@@ -1,4 +1,6 @@
-import Azurite.AzNat.Parse
+import Azurite.AzNat.Equiv.Basic
+import Azurite.AzNat.Basic
+import Azurite.AzNat.OfLimbs
 
 def UInt64.toAzNat (u : UInt64) : Azurite.AzNat :=
   if h : u = 0 then
@@ -27,23 +29,6 @@ def Int16.toAzNatClampNeg (i : Int16) : Azurite.AzNat := i.toInt64.toAzNatClampN
 def Int8.toAzNatClampNeg (i : Int8) : Azurite.AzNat := i.toInt64.toAzNatClampNeg
 def ISize.toAzNatClampNeg (i : ISize) : Azurite.AzNat := i.toInt64.toAzNatClampNeg
 
-#guard (0 : UInt64).toAzNat.toNat == 0
-#guard (5 : UInt64).toAzNat.toNat == 5
-#guard (18446744073709551615 : UInt64).toAzNat.toNat == 18446744073709551615
-
-#guard ((0 : Int64).toAzNatClampNeg).toNat == 0
-#guard ((-5 : Int64).toAzNatClampNeg).toNat == 0
-#guard ((-9223372036854775808 : Int64).toAzNatClampNeg).toNat == 0
-#guard ((5 : Int64).toAzNatClampNeg).toNat == 5
-#guard ((9223372036854775807 : Int64).toAzNatClampNeg).toNat == 9223372036854775807
-
-#guard ((0 : Int32).toAzNatClampNeg).toNat == 0
-#guard ((-5 : Int32).toAzNatClampNeg).toNat == 0
-#guard ((5 : Int32).toAzNatClampNeg).toNat == 5
-
-#guard ((-5 : ISize).toAzNatClampNeg).toNat == 0
-#guard ((5 : ISize).toAzNatClampNeg).toNat == 5
-
 namespace Azurite.AzNat
 
 def toUInt64 (n : AzNat) : UInt64 :=
@@ -61,20 +46,3 @@ def toInt8 (n : AzNat) : Int8 := n.toUInt64.toUInt8.toInt8
 def toISize (n : AzNat) : ISize := n.toUInt64.toUSize.toISize
 
 end Azurite.AzNat
-
-#guard (Azurite.AzNat.parse "123".toList).get!.toUInt64 == 123
-#guard (Azurite.AzNat.parse "18446744073709551617".toList).get!.toUInt64 == 1
-#guard (Azurite.AzNat.parse "18446744073709551616".toList).get!.toInt64 == 0
-#guard (Azurite.AzNat.parse "9223372036854775808".toList).get!.toInt64 == -9223372036854775808
-
-#guard (Azurite.AzNat.parse "4294967297".toList).get!.toUInt32 == 1
-#guard (Azurite.AzNat.parse "4294967295".toList).get!.toInt32 == -1
-#guard (Azurite.AzNat.parse "2147483648".toList).get!.toInt32 == -2147483648
-
-#guard (Azurite.AzNat.parse "65537".toList).get!.toUInt16 == 1
-#guard (Azurite.AzNat.parse "65535".toList).get!.toInt16 == -1
-#guard (Azurite.AzNat.parse "32768".toList).get!.toInt16 == -32768
-
-#guard (Azurite.AzNat.parse "257".toList).get!.toUInt8 == 1
-#guard (Azurite.AzNat.parse "255".toList).get!.toInt8 == -1
-#guard (Azurite.AzNat.parse "128".toList).get!.toInt8 == -128
