Azurite/AzNat/Tests/TrailingZeros.lean
@@ -1,0 +1,19 @@
+import Azurite.AzNat.ParseBase
+import Azurite.AzNat.TrailingZeros
+
+namespace Azurite.AzNat
+
+-- 0 has infinitely many trailing zeros
+#guard (AzNat.parse "0").get!.trailingZeros == none
+-- 1 = ...001₂, 0 trailing zeros
+#guard (AzNat.parse "1").get!.trailingZeros == some 0
+-- 8 = 1000₂, 3 trailing zeros
+#guard (AzNat.parse "8").get!.trailingZeros == some 3
+-- 12 = 1100₂, 2 trailing zeros
+#guard (AzNat.parse "12").get!.trailingZeros == some 2
+-- 2^64, so 64 trailing zeros
+#guard (AzNat.parse "18446744073709551616").get!.trailingZeros == some 64
+-- 3 * 2^128, so 128 trailing zeros
+#guard (AzNat.parse "1020847100762815390390123822295304634368").get!.trailingZeros == some 128
+
+end Azurite.AzNat
